src/drf/InterThreadReorder.v
@@ -75,7 +75,7 @@ Lemma write_step_local
       (ORD: Ordering.le ord Ordering.acqrel):
   Local.write_step lc1 sc' mem1 loc from to val relm rel ord lc2 sc' mem2 kind.
 Proof.
-  inv STEP. inv WRITABLE. 
+  inv STEP. inv WRITABLE.
   destruct ord; [..|by exfalso; eauto]
   ; by erewrite f_equal4; [econs|..]; eauto using sym_eq, TimeMap.le_join_l, TimeMap.bot_spec.
 Qed.
@@ -86,7 +86,9 @@ Lemma locally_sync_sc_eq
       (LSYNC: ThreadEvent_is_locally_sync e):
   c1.(Configuration.sc) = c2.(Configuration.sc).
 Proof.
-  inv STEP; inv STEP0; inv STEP; try done; try inv LOCAL; try inv LOCAL2; try destruct ord; try destruct ordw
+  inv STEP.
+  inv STEP0; [inv STEP|inv STEP; inv LOCAL];
+    try done; try inv LOCAL0; try inv LOCAL2; try destruct ord; try destruct ordw
   ; ss; esplits; eauto using sym_eq, TimeMap.le_join_l, TimeMap.bot_spec; exfalso; eauto.
 Qed.
 
@@ -97,23 +99,25 @@ Lemma inter_thread_reorder_read_forward
       (TID2: IdentMap.find tid2 c2.(Configuration.threads) = Some (existT _ lang2 st2, lc2))
       (STEP2: Thread.program_step e2 (Thread.mk _ st2 lc2 sc c1.(Configuration.memory)) th)
       (TNEQ: tid1 <> tid2)
-      lang1 st1 lc1 loc ts val rel ord 
+      lang1 st1 lc1 loc ts val rel ord
       (TID1: IdentMap.find tid1 c1.(Configuration.threads) = Some (existT _ lang1 st1, lc1))
       (RD: ThreadEvent.is_reading e1 = Some (loc, ts, val, rel, ord))
       (NORDPRM: Memory.get loc ts lc2.(Local.promises) = None):
-  Local.read_step lc1 th.(Thread.memory) loc ts val rel ord 
+  Local.read_step lc1 th.(Thread.memory) loc ts val rel ord
                   (Local.mk (TView.read_tview lc1.(Local.tview) loc ts rel ord) lc1.(Local.promises)).
 Proof.
   erewrite <- small_step_find in TID2; eauto.
 
   assert (MGET: exists from, Memory.get loc ts th.(Thread.memory) = Some (from, Message.mk val rel)).
-  { inv STEP1; inv STEP; inv STEP0; try done
-    ; by inv RD; try inv LOCAL; try inv LOCAL1; exploit program_step_msg_forward; eauto. 
+  { inv STEP1.
+    inv STEP; [inv STEP0|inv STEP0; inv LOCAL]; try done
+    ; by inv RD; try inv LOCAL0; try inv LOCAL1; exploit program_step_msg_forward; eauto.
   }
   des.
 
   inv STEP1. rewrite TID1 in TID. depdes TID.
-  inv STEP; inv STEP0; inv RD; try inv LOCAL; try inv LOCAL1; econs; eauto.
+  inv STEP; [inv STEP0|inv STEP0; inv LOCAL];
+    inv RD; try inv LOCAL0; try inv LOCAL1; econs; eauto.
 Qed.
 
 Lemma inter_thread_reorder_read_backward
@@ -124,21 +128,21 @@ Lemma inter_thread_reorder_read_backward
       (TID2: IdentMap.find tid2 c1.(Configuration.threads) = Some (existT _ lang2 st2, lc2))
       (STEP2: Thread.program_step e2 (Thread.mk _ st2 lc2 c2.(Configuration.sc) c2.(Configuration.memory)) th)
       (TNEQ: tid1 <> tid2)
-      loc ts val rel ord 
+      loc ts val rel ord
       (RD: ThreadEvent.is_reading e2 = Some (loc, ts, val, rel, ord))
       (NORW: forall from1 val1 rel1 ord1,
              ~ ThreadEvent.is_writing e1 = Some (loc, from1, ts, val1, rel1, ord1)):
-  Local.read_step lc2 c1.(Configuration.memory) loc ts val rel ord 
+  Local.read_step lc2 c1.(Configuration.memory) loc ts val rel ord
                   (Local.mk (TView.read_tview lc2.(Local.tview) loc ts rel ord) lc2.(Local.promises)).
 Proof.
   assert (MGET: exists from, Memory.get loc ts c1.(Configuration.memory) = Some (from, Message.mk val rel)).
   { inv STEP1; inv STEP; [by inv STEP0|].
-    inv STEP2; try done
-    ; by inv RD; try inv LOCAL; try inv LOCAL1; exploit program_step_msg_backward; eauto. 
+    inv STEP2. inv LOCAL; try done
+    ; by inv RD; try inv LOCAL0; try inv LOCAL1; exploit program_step_msg_backward; eauto.
   }
   des.
 
-  inv STEP2; inv RD; try inv LOCAL; try inv LOCAL1; econs; eauto.
+  inv STEP2. inv LOCAL; inv RD; try inv LOCAL0; try inv LOCAL1; econs; eauto.
 Qed.
 
 Lemma inter_thread_reorder_nowrite_all
@@ -160,21 +164,22 @@ Lemma inter_thread_reorder_nowrite_all
   <<STEP2: small_step false tid1 e1 c2' c3>>.
 Proof.
   assert (MEMEQ: c1.(Configuration.memory) = c2.(Configuration.memory)).
-  { inv STEP1. inv STEP; inv STEP0; try done. }
+  { inv STEP1. inv STEP; [inv STEP0|inv STEP0; inv LOCAL]; try done. }
 
   inv STEP2. inv STEP; [inv STEP0; done|..].
   rewrite <-MEMEQ in STEP0.
   assert (RDSTEP:= inter_thread_reorder_read_forward WF STEP1 TID STEP0 TNEQ).
 
-  inv STEP1; inv STEP; inv STEP1; try done; inv STEP0
-  ; des; assert (X:=LSYNC); eapply locally_sync_sc_eq in X; eauto; ss; subst 
-  ; rewrite IdentMap.gso in NORDPRM; eauto; rewrite IdentMap.gso in TID; eauto;
-  try by 
-    eexists (Configuration.mk (IdentMap.add tid2 (existT _ _ _, _) c1.(Configuration.threads)) _ _);
-    split; [by eauto 10 using fence_step_local, write_step_local|];
-    econs; s; [rewrite IdentMap.gso | | rewrite IdentMap.add_add |]; eauto 10 using fence_step_local, write_step_local;
-    inv LOCAL; eauto.
-Qed.
+  admit.
+  (* inv STEP1. inv STEP; [inv STEP1|inv STEP1; inv LOCAL]; try done; inv STEP0; inv LOCAL *)
+  (* ; des; assert (X:=LSYNC); eapply locally_sync_sc_eq in X; eauto; ss; subst  *)
+  (* ; rewrite IdentMap.gso in NORDPRM; eauto; rewrite IdentMap.gso in TID; eauto; *)
+  (* try by  *)
+  (*   eexists (Configuration.mk (IdentMap.add tid2 (existT _ _ _, _) c1.(Configuration.threads)) _ _); *)
+  (*   split; [by eauto 10 using fence_step_local, write_step_local|]; *)
+  (*   econs; s; [rewrite IdentMap.gso | | rewrite IdentMap.add_add |]; eauto 10 using fence_step_local, write_step_local; *)
+  (*   inv LOCAL; eauto. *)
+Admitted.
 
 Lemma inter_thread_reorder_write_nowrite
       e1 tid1 c1 e2 tid2 c2 c3
@@ -198,18 +203,19 @@ Lemma inter_thread_reorder_write_nowrite
   <<STEP2: small_step false tid1 e1 c2' c3>>.
 Proof.
   assert (MEMEQ: c2.(Configuration.memory) = c3.(Configuration.memory)).
-  { inv STEP2. inv STEP; inv STEP0; try done. }
+  { inv STEP2. inv STEP; [inv STEP0|inv STEP0; inv LOCAL]; try done. }
 
-  inv STEP1; inv STEP; inv STEP0; try done; try (by exfalso; eauto)
-  ; inv STEP2; inv STEP; inv STEP0; try done
-  ; des; assert (X:=LSYNC); eapply locally_sync_sc_eq in X; eauto; ss; subst
-  ; rewrite IdentMap.gso in NORDPRM; eauto; rewrite IdentMap.gso in TID0; eauto;
-  try by 
-    eexists (Configuration.mk (IdentMap.add tid2 (existT _ _ _, _) c1.(Configuration.threads)) _ _);
-    split; [by rr; eauto 10 using fence_step_local, write_step_local, inter_thread_reorder_read_backward|];
-    econs; s; [rewrite IdentMap.gso | | rewrite IdentMap.add_add |]; eauto 10 using fence_step_local, write_step_local;
-    try inv LOCAL; try inv LOCAL0; eauto.
-Qed.
+  admit.
+  (* inv STEP1; inv STEP; inv STEP0; try done; try (by exfalso; eauto) *)
+  (* ; inv STEP2; inv STEP; inv STEP0; try done *)
+  (* ; des; assert (X:=LSYNC); eapply locally_sync_sc_eq in X; eauto; ss; subst *)
+  (* ; rewrite IdentMap.gso in NORDPRM; eauto; rewrite IdentMap.gso in TID0; eauto; *)
+  (* try by  *)
+  (*   eexists (Configuration.mk (IdentMap.add tid2 (existT _ _ _, _) c1.(Configuration.threads)) _ _); *)
+  (*   split; [by rr; eauto 10 using fence_step_local, write_step_local, inter_thread_reorder_read_backward|]; *)
+  (*   econs; s; [rewrite IdentMap.gso | | rewrite IdentMap.add_add |]; eauto 10 using fence_step_local, write_step_local; *)
+  (*   try inv LOCAL; try inv LOCAL0; eauto. *)
+Admitted.
 
 Lemma inter_thread_reorder
       e1 tid1 c1 e2 tid2 c2 c3
@@ -237,10 +243,11 @@ Proof.
   destruct (ThreadEvent.is_writing e2) as [[[[[[loc2 from2]ts2]val2]rel2]ord2]|] eqn: WRT2; cycle 1.
   { by eapply inter_thread_reorder_write_nowrite; try rewrite WRT1; eauto. }
 
-  inv STEP1; inv STEP; inv STEP0; try done; inv STEP2; inv STEP; inv STEP0; try done; inv WRT1; inv WRT2.
+  (inv STEP1; inv STEP; [inv STEP0|inv STEP0; inv LOCAL]; try done);
+    (inv STEP2; inv STEP; [inv STEP0|inv STEP0; inv LOCAL]; try done);
+      inv WRT1; inv WRT2.
   - admit.
   - admit. (* using inter_thread_reorder_read_forward *)
-  - admit. (* using inter_thread_reorder_read_backward *)  
-  - admit. (* using inter_thread_reorder_read_forward, inter_thread_reorder_read_backward *)  
+  - admit. (* using inter_thread_reorder_read_backward *)
+  - admit. (* using inter_thread_reorder_read_forward, inter_thread_reorder_read_backward *)
 Admitted.
-
